

\append{Transpose of Full Acoustic Modeling Operator}
In this section I compute the adjoint operator form modeling with both pressure and velocity source inputs and pressure and velocity trace outputs. The forward modeling operator is defined by solving
\begin{eqnarray}
\label{eqn:fawedata}
\frac{\partial p}{\partial t} & = & - \kappa( \nabla \cdot \bv +
h_s \delta(z-z_s)), \nonumber \\
\frac{\partial \bv}{\partial t} & = & - \beta ( \nabla p + l_s {\bf e}_z\delta(z-z_s)),\nonumber \\
p & =& 0 \mbox{ for } t<0\nonumber\\ 
\bv & = & 0 \mbox{ for } t<0 \nonumber\\
\end{eqnarray}
The new elements here are the point load time function $l_s(\bx,t;\bx_s)$, and the vertical unit vector ${\bf e}_z=(0,1)^T$ for 2D, $=(0,0,1)^T$ for 3D. The forward map ${\bf F}$ is defined as implicit in the discussion of the Intrinsically Preconditioned CG algorithm: let ${\bf h}_s=(h_s,l_s)^T$, then 
\begin{equation}
\label{eqn:ffwd}
{\bf F}{\bf h}_s =\left\{ \left[
\begin{array}{c}
p(\bx,t;\bx_s)\\
v_z(\bx,t;\bx_s)
\end{array}
\right]_{z=z_r}\right\}
\end{equation}

Let $\tilde{\bf h}_r=(\tilde{h}_r,\tilde{l}_r)^T$ be a function on $z=z_r$, 
and 
$\tilde{p},\tilde{\bv}$ solve the backwards-in-time boundary value problem:
\begin{eqnarray}
\label{eqn:faweadj}
\frac{\partial \tilde{p}}{\partial t} & = & \kappa (-\nabla \cdot \tilde{\bv} + 
 \tilde{h}_r \delta(z-z_r))\nonumber \\
\frac{\partial \tilde{\bv}}{\partial t} & = & \beta (\nabla \tilde{p} + \tilde{l}_r{\bf e}_z\delta(z-z_r),\nonumber \\
\tilde{p} & =& 0 \mbox{ for } t>T\nonumber\\ 
\tilde{\bv} & = & 0 \mbox{ for } t>T 
\end{eqnarray} 
Then
\[
0 = 
\left(\int\, dx\,dy\,dz\, \frac{p \tilde{p}}{\kappa} +  
\frac{\bv \cdot \tilde{\bv}}{\beta} \right)|_{t=T}
-
\left(\int\, dx\,dy\,dz\, \frac{p \tilde{p}}{\kappa} +  \frac{\bv \cdot \tilde{\bv}}{\beta} \right)|_{t=0}
\]
\[
= 
\int_{0}^{T} \,dt\, \frac{d}{dt}\left(\int\, dx\,dy\,dz\, \frac{p \tilde{p}}{\kappa} +  \frac{\bv \cdot \tilde{\bv}}{\beta} \right)
\]
\[
= 
\int_{0}^{T} \,dt\, \left(\int\, dx\,dy\,dz\, \frac{1}{\kappa} \frac{\partial p}{\partial t} \tilde {p} +  p \frac{1}{\kappa}\frac{\partial \tilde{p}}{\partial t} \right.
\]
\[
+
\left. \frac{1}{\beta} \frac{\partial \bv}{\partial t} \cdot \tilde{\bv} + \frac{1}{\beta} \bv \cdot \frac{\partial \tilde{\bv}}{\partial t} \right)
\]
\[
= 
\int_{0}^{T} \,dt\, \left(\int\, dx\,dy\,dz\, \left(- \nabla \cdot \bv + 
 h_s \delta(z-z_s)\right) \tilde{p} + p \left(- \nabla \cdot \tilde{\bv} + 
 \tilde{h}_r \delta(z-z_r)\right) \right.
\]
\[
+
\left.  (- \nabla p + l_s{\bf e}_z\delta(z-z_s)) \cdot \tilde{\bv} + \bv \cdot (-\nabla \tilde{p} + \tilde{l}_r{\bf e}_z\delta(z-z_r)) \right)
\]
\[
= 
\int_{0}^{T}\,dt\, \left(\int\, dx\,dy\,dz\, \left(- \nabla \cdot \bv \tilde{p} + 
 h_s\tilde{p}|_{z=z_s} - p\nabla \cdot \tilde{\bv} + 
 \tilde{h}_r p|_{z=z_r}\right) \right.
\]
\[
+
\left.  p (\nabla \cdot \tilde{\bv}) + l_s \tilde{v}_z|_{z=z_r}+ (\nabla \cdot \bv) \tilde{p}  + l_r  v_z|_{z=z_r}\right)
\]
after integration by parts in the last two terms. Most of what is left cancels, leaving 
\[
0 = \int\,dt\,dx\,dy\, (h_s \tilde{p})_{z=z_s} + (p  \tilde{h}_r)_{z=z_r} + (l_s\tilde{v}_z)_{z=z_s} + (v_z \tilde{l}_r)_{z=z_r},
\]
whence
\begin{equation}
\label{eqn:fadj}
 {\bf F}^T {\bf h}_r = -\left[
\begin{array}{c}
\tilde{p}(\bx,t;\bx_s)\\
\tilde{\bf v}(\bx,t;\bx_s)
\end{array}
\right]_{z=z_s}
\end{equation}

%\begin{cor}\label{thm:bvps}
%Suppose that $d_s$ is a sufficiently regular function, = 0 for $t<0$, and denote by $p^{\pm},\bv^{\pm}$ the half-space solutions provided by Theorem \ref{thm:bvp}. Define the vector fields $p,\bv$ in $\bR^4$ by
%\begin{eqnarray}
%\label{eqn:putemtogether} 
%p(x,z) &=& p^{\pm}(x,z) \mbox{ for } \pm(z-z_s) > 0\\
%p(x,z_s)&=&d_s(x)\\
%\bv(x,z) &=& \bv^{\pm}(x,z) \mbox{ for } \pm(z-z_s) > 0\\
%\end{eqnarray}
%Then $p,\bv$ is a weak solution of the system \ref{eqn:awedata} with $h=[v]_n$.
%\end{cor}

Proof of Theorem \ref{thm:bvp}:

\begin{proof}
Since $\omega \cap \mbox{ supp }d$ is compact, it is possible to construct an extension of 
$d \in C^{\infty}_{0}(\bR^{d+1})$. Define $p_1^{\pm}, \bv_1^{\pm}$ to be strong solutions of the system
\begin{eqnarray}
\label{eqn:ichom}
\frac{\partial p^{\pm}_1}{\partial t} & = & - \kappa \nabla \cdot \bv^{\pm}_1 + F\mbox{ in } \Omega^{\pm}, \nonumber \\
\frac{\partial \bv^{\pm}_1}{\partial t} & = & - \beta \nabla p^{\pm}_1 + {\bf G}\mbox{ in } \Omega^{\pm},\nonumber \\
p^{\pm}_1 & = & 0 \mbox{ on } \omega \times \bR,\\
p^{\pm}_1 & = & 0, t \ll 0\\
\bv^{\pm}_1 & = & 0, t \ll 0 
\end{eqnarray}
with 
\[
F = -\gamma\frac{\partial d}{\partial t}, {\bf G} = -\nabla d.
\]
Existence, uniqueness, and regularity of these solutions are assured by a minor extension of results of \cite{BlazekStolkSymes:13}.
Set $p^{\pm} = p_1^{\pm} + d, \bv^{\pm} = \bv_1^{\pm}$; then $p^{\pm},\bv^{\pm}$ are the unique strong solutions of the boundary value problems \ref{eqn:awebdry}, and are smooth up to the boundary as indicated. 
\end{proof}

Proof of Corollary \ref{thm:bvps}:

\begin{proof}: Choose smooth functions $\phi \in C^{\infty}_0(\bR^{d+1}), {\bf \psi} \in  (C^{\infty}_0(\bR^{d+1}))^d$. Then
\[
\int_{\Omega^{\pm} \times \bR}\left (\gamma \frac{\partial \phi}{\partial t} +
\nabla \cdot {\bf \psi}\right)p^{\pm} + \left(\rho\frac{\partial {\bf
    \psi}}{\partial t}
  + \nabla \phi\right) \cdot \bv^{\pm}
\]
\[
= - \int_{\Omega \times \bR}\left (\gamma \frac{\partial p^{\pm}}{\partial t} +
\nabla \cdot \bv^{\pm}\right) \phi + \left(\rho\frac{\partial \bv^{\pm}}{\partial t}
  + \nabla p^{\pm}\right) \cdot {\bf \psi}
\]
\begin{equation}
\label{eqn:rhs1}
\pm \int_{\omega \times \bR} \bn \cdot {\bf \psi} p^{\pm} + \bn
  \cdot \bv^{\pm} \phi
\end{equation}
Adding equations \ref{eqn:rhs1} for the two choices of sign and taking into
account that $p^{\pm}$ coincide (by construction) on $\omega \times \bR$, obtain
\[
\int_{(\bR^d \times \bR}\left (\gamma \frac{\partial \phi}{\partial t} +
\nabla \cdot {\bf \psi}\right)p + \left(\rho\frac{\partial {\bf
    \psi}}{\partial t}
  + \nabla \phi\right) \cdot \bv
\]
\[
= \int_{\partial \Omega \times [0,T]} (\bn \cdot \bv^{+} -  \bn
  \cdot \bv^{-}) \phi
\]
Since $\phi$ and ${\bf \psi}$ are arbitrary, other than being smooth of compact support, this observation finishes the proof.
\end{proof}
