\title{Convergent DSO Gradient Computation}

\author{
William Symes\thanks{Department of Computational and Applied Mathematics, Rice University,
Houston, TX, 77005, USA,
{\tt symes@rice.edu}}
}

\lefthead{Symes}

\righthead{DSO Gradient}

\maketitle
\parskip 12pt

\begin{abstract}
A really short abstract.
\end{abstract}

\section{Introduction} 

\section{VPM for extended FWI}

$M$ = model space (macro models)

$\oM$ = extended model space (perturbations)

$D$ = data space

$\oF: M \rightarrow {\cal L}(\oM, D)$ = extended Born modeling operator

$A: \oM \rightarrow \oM$ = annihilator

Inner products: 
\begin{itemize}
\item $\langle \dom_1,\dom_2\rangle_m = \dom_1^T W_m{\color{blue}[m]}\dom_2$ in $\oM$
\item $\langle d_1,d_2 \rangle_d = d_1^T W_d d_2$ in $D$, 
\item $\langle m_1,m_2\rangle_b = m_1^TW_b m_2 $ in $M$
\end{itemize}

$\odF$ = adjoint of $\oF$ (wrt inner products in $\oM$, $D$) = $W_m^{-1}\oF^TW_d$, etc.

Variable Projection objective
\[
\Ja[m,\dd] = \mbox{min}_{\dom} \frac{1}{2}(\|\oF[m]\dom -\dd\|_d^2 + \alpha^2\|A\dom\|_m^2)
\]
\[
= \frac{1}{2}(\|\oF[m]\dom[m] -\dd\|_d^2 + \alpha^2\|A\dom[m]\|^2)
\]
$\dom[m]$ = solution of normal equation  
\[
\Na[m] \dom[m] = \odF[m] \dd,\,\,\Na[m] = \odF[m]\oF[m] + \alpha^2 A^{\dagger}A
\]

Variable Projection Method:
\[
D\Ja[m,\dd]\delta m = \langle D\oF[m](\delta m,\dom[m]), \oF[m]\dom[m]-\dd\rangle_d
\]
\[
= \langle \delta m, D\oF[m]^*(\dom[m],\oF[m]\dom[m]-\dd) \rangle_b
\]
for any $\delta m \in M$ $\Rightarrow$
\[
\nabla_m \Ja[m,\dd] = D\oF[m]^*(\dom[m],\oF[m]\dom[m]-\dd)
\]

\section{Problem}
Normal equation must be solved by iterative method:
\[
\dom_a \rightarrow \dom[m],\, a \rightarrow \infty
\]
meaning $\|\dom_a-\dom[m]\|_m \rightarrow 0$.

However $D\oF[m]$ is not $\oM$-continuous:
\[
\dom_a \rightarrow \dom[m] \mbox{ does not imply } DF[m](\delta m,\dom_a) \rightarrow DF[m](\delta m, \dom[m])
\]


Example: extended acoustic Born modeling, $m=$ velocity, $\dom(\bx,\bh)$ = extended velocity perturbation, $\phi = T(\bx_r,\bx+\bh)-T(\bx_s,\bx-\bh)$
\[
\oF[m]\dom(\bx_r,t;\bx_s)  \approx \partial_t^2 \int d\bx d\bh A \delta(t-\phi) \dom
\]
\[
D\oF[m](\delta m,\dom) (\bx_r,t;\bx_s) \approx \partial_t^2 \int d\bx d\bh A
\partial_t \delta(t-\phi)(-D\phi \delta m)\dom
\]
\[
 \approx \partial_t^2 \int d\bx d\bh A\partial_z\delta(t-\phi)\frac{D\phi \delta m}{\partial_z \phi} \dom
 \approx \partial_t^2 \int d\bx d\bh A\delta(t-\phi)\frac{D\phi \delta m}{\partial_z \phi}{\color{blue} \partial_z} \dom
 \]
 \[
\dom_a \rightarrow \dom[m] \mbox{ does not imply } \partial_z \dom_a \rightarrow \partial_z \dom[m]
\]

\section{Solution: $\oF$ is unitary modulo smoothing}

Assumption: $\oF$ {\em asymptotically unitary} wrt $\oM, D$ norms: $\odF\oF = I + S$, 

$S$ is (at least) 1-smoothing: $\dom_a \rightarrow \dom_0$ $\Rightarrow$ $P S \dom_a \rightarrow  P S\dom_0$, any $P \in OPS^1$

Examples: source-receiver extension (non-caustic case), full aperture scattering, but no other relevant examples for exploration

BUT easiest to understand concept in this case

VPM derivative:
\[
D\Ja[m,\dd]\delta m = \langle D\oF[m](\delta m,\dom[m]), \oF[m]\dom[m]-\dd\rangle_d
\]
\[
= \langle D\oF[m](\delta m,\dom[m]),\oF[m]\dom[m]\rangle_d -\langle D\oF[m](\delta m,\dom[m]),\dd\rangle_d
\]
\[
= {\bf 1} + {\bf 2}
\]
\[
{\bf 1} = \frac{1}{2}D\|\oF[m]\dom[m_1]\|^2(\delta m)_{m_1=m} = \frac{1}{2}\langle \dom[m], D(\odF[m]\oF[m])(\delta m, \dom[m])\rangle_m
\]
$\odF\oF$ is $\Psi$DO order 0 $\Rightarrow$ smoothly dependent on $m$ $\Rightarrow$ if $\dom_a \rightarrow \dom[m]$ then
\[
\langle D\oF[m](\delta m,\dom_a),\oF[m]\dom_a\rangle_d \rightarrow \langle D\oF[m](\delta m,\dom[m]),\oF[m]\dom[m]\rangle_d 
\]

Normal equation:
\[
\Na[m] \dom[m] = \odF[m] \dd, \,\,\Na = \odF[m]\oF[m] +\alpha^2  A^{\dagger}A = I + \alpha^2 A^{\dagger}A + S[m]
\]

\[
\Rightarrow \dom[m] = (I + \alpha^2 A^{\dagger}A)^{-1}(\odF[m]\dd -S[m]\dom[m]) 
\]

\[
{\bf 2} = -\langle D\oF[m](\delta m,(I + \alpha^2 A^{\dagger}A)^{-1}(\odF[m]\dd)),\dd\rangle_d 
\]

\[
+ \langle D\oF[m](\delta m, (I+\alpha^2 A^{\dagger}A)^{-1}S[m]\dom[m]),\dd\rangle_d
\]

$(I+\alpha^2 A^{\dagger}A)^{-1}S[m]$ also 1-smoothing 

\[
L_a (\delta m,\dom_a) = \langle D\oF[m](\delta m,\dom_a),\oF[m]\dom_a\rangle_d 
\]
\[
+ \langle D\oF[m](\delta m, (I+\alpha^2 A^{\dagger}A)^{-1}S[m]\dom_a),\dd\rangle_d
\]
\[
-\langle D\oF[m](\delta m,(I + \alpha^2 A^{\dagger}A)^{-1}(\odF[m]\dd)),\dd\rangle_d 
\]

Convergent derivative approximation:

$\dom_a \rightarrow \dom[m]$ $\Rightarrow$ $L_a(\delta m, \dom_a) \rightarrow D\Ja[m,\dd]\delta m$

Gradient:
\[
L_a(\delta m, \dom_a) = \langle \delta m, G_a(\dom_a) \rangle,
\]

\[
G_a(\dom_a) = D\oF[m]^*(\dom_a,\oF[m]\dom_a) 
\]
\[
- D\oF[m]^*((I+\alpha^2 A^{\dagger}A)^{-1}(\odF[m]\dd -S[m]\dom_a),\dd) 
\]

$G_a$ $\oM-$continuous $\Rightarrow$ 

$\dom_a \rightarrow \dom[m]$ $\Rightarrow$ $G_a(\dom_a) \rightarrow \nabla_m \Ja[m,\dd]$

Computationally convenient rewrite:
\[
S = \Na - (I+\alpha^2 A^{\dagger}A) \Rightarrow \odF\dd-S\dom_a = g_a + (I+\alpha^2 A^{\dagger}A)\dom_a
\]

\[
g_a = \odF \dd - \Na\dom_a = \mbox{ normal residual }
\]

\[
G_a(\dom_a) = D\oF[m]^*(\dom_a,\oF[m]\dom_a) 
\]
\[
- D\oF[m]^*((I+\alpha^2 A^{\dagger}A)^{-1}g_a +\dom_a,\dd) 
\]

\[
= D\oF[m]^*(\dom_a,\oF[m]\dom_a-\dd) - D\oF[m]^*((I+\alpha^2 A^{\dagger}A)^{-1}g_a,\dd)
\]
